the ms table is indexed both by id and rid

src/tls/MasterSecret.fst
@@ -8,23 +8,34 @@ let tls_region = new_region root
 module AE = StreamAE
 module MM = MonotoneMap
 module MR = FStar.Monotonic.RRef
+module HH = FStar.HyperHeap
 
-let ms_tab : MM.t tls_region AE.id AE.writer (fun x -> True) =
-  MM.alloc #tls_region #AE.id #AE.writer #(fun x -> True)
+type writer (ids:(AE.id * rid)) = w:AE.writer (fst ids){HH.extends (StreamAE.State.region w) (snd ids)}
+let ids = (AE.id * rid)
+let map_invariant (m:MM.map' ids writer) = True
+  (* Failed attempt *)
+  (* (forall i1 i2. is_Some (m i1) /\ is_Some (m i2) /\ fst i1 = fst i2 ==> i1 = i2) *)
+  (* /\ (forall i. is_None (m i) ==> (forall j. fst i = fst j ==> is_None (m j))) *)
+
+let ms_tab : MM.t tls_region ids writer map_invariant = 
+  MM.alloc #tls_region #ids #writer #map_invariant
+
+assume val gcut: f:(unit -> GTot Type){f()} -> Tot unit
+assume val gadmit: f:(unit -> GTot Type) -> Tot (u:unit{f()})
 
 let derive (r:rid) (i:AE.id) 
   : ST (AE.writer i)
        (requires (fun h -> disjoint r tls_region))
        (ensures (fun h0 w h1 -> 
-	   (* StreamAE.State.region w = r *) //not yet sure how to prove this part
-	   (* /\  *)modifies (Set.singleton tls_region) h0 h1
-	   /\ MR.witnessed (MM.t_contains ms_tab i w)))
+	   HH.extends (StreamAE.State.region w) r 
+	   /\ modifies (Set.singleton tls_region) h0 h1
+	   /\ MR.witnessed (MM.t_contains ms_tab (i,r) w)))
   = recall_region tls_region;
-    let y = MM.lookup ms_tab i in
+    let y = MM.lookup ms_tab (i, r) in
     match y with 
     | None -> 
       let w = AE.gen r i in 
-      MM.extend ms_tab i w;
+      MM.extend ms_tab (i,r) w;
       w
     | Some w -> 
       w
